\documentclass[fleqn]{article}
\usepackage{amsmath}

\begin{document}
\thispagestyle{empty}

\subsection*{Definitions}
\noindent
We find the derivative of $f{^{-1} (x)} = \tan^{-1}{x}$ by applying the Theorm of derivation of inverse functions.
\newline

\begin{align*}
    \left(f{^{-1}}\right){^{\prime}}(x) =& \frac{1}{f{^{\prime} \left(f{^{-1}}(x)\right)}} \\
    =& \frac{1}{\sec{^2 \left(\tan{^{-1}}{x}\right)}} \qquad\qquad f{^{\prime} (u)} = \sec{^2 u} \\
    =& \frac{1}{1 + \tan{^{2} \left(\tan{^{-1} x}\right)}} \qquad \sec{^2 u} = 1 + \tan{^2 u} \\
    =& \frac{1}{1 + x{^2}} \qquad\qquad\qquad\quad  \tan{\left(\tan{^{-1} x}\right)} = x
\end{align*}

\noindent
So, the general rule for derivative of $\tan{^{-1} u}$ is:
\newline

\begin{align*}
    \frac{d}{dx}\left(\tan{^{-1} u}\right) = \frac{1}{1 + u^2}\frac{du}{dx}
\end{align*}

\subsection*{Excerises}
\noindent
Find the derivatives of the following exercises:
\newline

\begin{align*}
1.\;&\ln{\left(\tan{^{-1} x}\right)} \\
2.\;&\tan{^{-1} \left(\ln{x}\right)}
\end{align*}

\end{document}
